
c_{haosGameIter}\left(x,c_{hoices},r_{ands}\right)=\frac{\left(c_{hoices}\left[\left(1+r_{ands}\right)\right]+x\right)}{2}
i=0
x_{Pos}=\left(0+\left(0*\left[1,...,9000\right]\right)\right)
y_{Pos}=\left(0+\left(0*\left[1,...,9000\right]\right)\right)
z_{Pos}=\left(5.5+\left(0*\left[1,...,9000\right]\right)\right)
x_{PosRotated1}=\left(\left(x_{Pos}*\operatorname{cos}\left(r_{otation}.x\right)\right)-\left(z_{Pos}*\operatorname{sin}\left(r_{otation}.x\right)\right)\right)
y_{PosRotated1}=y_{Pos}
z_{PosRotated1}=\left(\left(x_{Pos}*\operatorname{sin}\left(r_{otation}.x\right)\right)+\left(z_{Pos}*\operatorname{cos}\left(r_{otation}.x\right)\right)\right)
x_{PosRotated}=x_{PosRotated1}
y_{PosRotated}=\left(\left(y_{PosRotated1}*\operatorname{cos}\left(r_{otation}.y\right)\right)-\left(z_{PosRotated1}*\operatorname{sin}\left(r_{otation}.y\right)\right)\right)
z_{PosRotated}=\left(\left(y_{PosRotated1}*\operatorname{sin}\left(r_{otation}.y\right)\right)+\left(z_{PosRotated1}*\operatorname{cos}\left(r_{otation}.y\right)\right)\right)
r_{andoms}=\operatorname{floor}\left(\left(4*\operatorname{random}\left(9000\right)\right)\right)
x_{Points}=\left[-1,1,-1,-1\right]
y_{Points}=\left[-1,-1,1,-1\right]
z_{Points}=\left[-1,-1,-1,1\right]
d_{isplay}=\left(\frac{x_{PosRotated}}{\left(z_{PosRotated}+5\right)},\frac{y_{PosRotated}}{\left(z_{PosRotated}+5\right)}\right)
r_{otation}=\left(r_{otationController}*30\right)
r_{otationController}=\left(0,0\right)

m_{ain}\left(\right)=\left\{p_{c}=0:\left(\left\{i<10:p_{c}\to \left(p_{c}+1\right),p_{c}\to 6\right\}\right),p_{c}=1:\left(r_{andoms}\to \operatorname{floor}\left(\left(4*\operatorname{random}\left(9000\right)\right)\right),p_{c}\to \left(p_{c}+1\right)\right),p_{c}=2:\left(x_{Pos}\to c_{haosGameIter}\left(x_{Pos},x_{Points},r_{andoms}\right),p_{c}\to \left(p_{c}+1\right)\right),p_{c}=3:\left(y_{Pos}\to c_{haosGameIter}\left(y_{Pos},y_{Points},r_{andoms}\right),p_{c}\to \left(p_{c}+1\right)\right),p_{c}=4:\left(z_{Pos}\to c_{haosGameIter}\left(z_{Pos},z_{Points},r_{andoms}\right),p_{c}\to \left(p_{c}+1\right)\right),p_{c}=5:\left(i\to \left(i+1\right),p_{c}\to 0\right),p_{c}=6:\left(\left(p_{c}\to p_{s}\left[\operatorname{length}\left(p_{s}\right)\right],p_{s}\to p_{s}\left[1...\left(\operatorname{length}\left(p_{s}\right)-1\right)\right]\right)\right)\right\}
p_{s}=\left[-1\right]

p_{c}=0
