
c_{haosGameIter}\left(d_{ata}\right)=\operatorname{join}\left(\frac{\left(\left[p_{oints}\left[\left(1+\left(3*r_{andoms}\left[d_{ata}\left[4\right]\right]\right)\right)\right],p_{oints}\left[\left(2+\left(3*r_{andoms}\left[d_{ata}\left[4\right]\right]\right)\right)\right],p_{oints}\left[\left(3+\left(3*r_{andoms}\left[d_{ata}\left[4\right]\right]\right)\right)\right]\right]+d_{ata}\left[1...3\right]\right)}{2},\left(d_{ata}\left[4\right]+1\right)\right)
c_{haosGameIter10}\left(d_{ata}\right)=c_{haosGameIter}\left(c_{haosGameIter}\left(c_{haosGameIter}\left(c_{haosGameIter}\left(c_{haosGameIter}\left(c_{haosGameIter}\left(c_{haosGameIter}\left(c_{haosGameIter}\left(c_{haosGameIter}\left(c_{haosGameIter}\left(d_{ata}\right)\right)\right)\right)\right)\right)\right)\right)\right)\right)

i=0
r_{andoms}=\operatorname{floor}\left(\left(4*\operatorname{random}\left(10\right)\right)\right)
p_{oints}=\left[-1,-1,5,1,-1,5,-1,1,5,-1,-1,6\right]
c_{urrentPoint}=\left[0.5,0.5,5.5\right]
d_{isplay}=\left[\right]
d_{isplayCache}=\left[\right]

m_{ain}\left(\right)=\left\{p_{c}=0:\left(\left\{2>1:p_{c}\to \left(p_{c}+1\right),p_{c}\to 4\right\}\right),p_{c}=1:\left(\left(r_{andoms}\to \operatorname{floor}\left(\left(4*\operatorname{random}\left(10\right)\right)\right),c_{urrentPoint}\to c_{haosGameIter10}\left(\left[0.5,0.5,5.5,1\right]\right),d_{isplayCache}\to \operatorname{join}\left(d_{isplayCache},\left[\left(\frac{c_{urrentPoint}\left[1\right]}{c_{urrentPoint}\left[3\right]},\frac{c_{urrentPoint}\left[2\right]}{c_{urrentPoint}\left[3\right]}\right)\right]\right),i\to \left(i+1\right)\right),p_{c}\to \left(p_{c}+1\right)\right),p_{c}=2:\left(\left\{i>50:\left(\left(i\to 0,d_{isplay}\to \operatorname{join}\left(d_{isplay},d_{isplayCache}\right),d_{isplayCache}\to \left[\right]\right),p_{c}\to \left(p_{c}+1\right)\right),p_{c}\to 3\right\}\right),p_{c}=3:\left(i\to i,p_{c}\to 0\right),p_{c}=4:\left(\left(p_{c}\to p_{s}\left[\operatorname{length}\left(p_{s}\right)\right],p_{s}\to p_{s}\left[1...\left(\operatorname{length}\left(p_{s}\right)-1\right)\right]\right)\right)\right\}
p_{s}=\left[-1\right]

p_{c}=0
